Slightly more manageable encoding.

SystemF.dfy
@@ -81,6 +81,7 @@ function ty_size(T: ty): nat
   case TArrow(T1, T2) => 1+ty_size(T1)+ty_size(T2)
   case TBase => 1
 }
+
 function ty_fv(T: ty): set<int> //of free variables of T
 {
   match T
@@ -91,6 +92,18 @@ function ty_fv(T: ty): set<int> //of free variables of T
   case TArrow(T1, T2) => ty_fv(T1)+ty_fv(T2)
   case TBase => {}
 }
+function ty_tm_fv(t: tm): set<int> //of free type variables of t
+{
+  match t
+  // interesting cases...
+  case tyabs(x, body) => ty_tm_fv(body)-{x}
+  // congruent cases...
+  case tvar(id) => {}
+  case tabs(x, T, body) => ty_fv(T)+ty_tm_fv(body)
+  case tapp(f, arg) => ty_tm_fv(f)+ty_tm_fv(arg)
+  case tyapp(tf, targ) => ty_tm_fv(tf)+ty_fv(targ)
+}
+
 function not_in(s: set<int>, r: nat): nat
 {
   if (!exists x :: x in s) then r+1 else
@@ -98,8 +111,107 @@ function not_in(s: set<int>, r: nat): nat
   if (x<r) then not_in(s-{x}, r) else not_in(s-{x}, r)
 }
 
-function ty_ty_subst(X: int, S: ty, T: ty, L: set<int>): ty //[X -> S]T
-  ensures S.TVar? ==> ty_size(ty_ty_subst(X, S, T, L))==ty_size(T);
+function ty_var_swap(X: int, Y: int, Z: int): int
+{
+  if X==Z then Y else if Y==Z then X else Z
+}
+ghost method sym_ty_var_swap(X: int, Y: int, Z: int)
+  ensures ty_var_swap(X, Y, Z)==ty_var_swap(Y, X, Z);
+{
+}
+function ty_ty_swap(X: int, Y: int, T: ty): ty
+  ensures ty_size(T)==ty_size(ty_ty_swap(X, Y, T));
+{
+  match T
+  case TVar(X') => TVar(ty_var_swap(X, Y, X'))
+  case TForall(X', body) => TForall(ty_var_swap(X, Y, X'), ty_ty_swap(X, Y, body))
+  case TArrow(T1, T2) => TArrow(ty_ty_swap(X, Y, T1), ty_ty_swap(X, Y, T2))
+  case TBase => TBase
+}
+ghost method sym_ty_ty_swap(X: int, Y: int, T: ty)
+  ensures ty_ty_swap(X, Y, T)==ty_ty_swap(Y, X, T);
+{
+}
+function ty_tm_swap(X: int, Y: int, t: tm): tm
+{
+  match t
+  case tyabs(X', body) => tyabs(ty_var_swap(X, Y, X'), ty_tm_swap(X, Y, body))
+  case tvar(x) => t
+  case tabs(x, T, t1) => tabs(x, ty_ty_swap(X, Y, T), ty_tm_swap(X, Y, t1))
+  case tapp(t1, t2) => tapp(ty_tm_swap(X, Y, t1), ty_tm_swap(X, Y, t2))
+  case tyapp(tf, targ) => tyapp(ty_tm_swap(X, Y, tf), ty_ty_swap(X, Y, targ))
+}
+ghost method sym_ty_tm_swap(X: int, Y: int, t: tm)
+  ensures ty_tm_swap(X, Y, t)==ty_tm_swap(Y, X, t);
+{
+  if (t.tabs?) {
+    sym_ty_ty_swap(X, Y, t.T);
+  } else if (t.tyapp?) {
+    sym_ty_ty_swap(X, Y, t.targ);
+  }
+}
+
+predicate ty_eq(T1: ty, T2: ty)
+  ensures ty_eq(T1, T2) ==> ((T1.TArrow? <==> T2.TArrow?) &&
+                             (T1.TBase? <==> T2.TBase?) &&
+                             (T1.TVar? <==> T2.TVar?) &&
+                             (T1.TForall? <==> T2.TForall?) &&
+                             ((T1.TArrow? && T2.TArrow?) ==> (ty_eq(T1.T1, T2.T1) && ty_eq(T1.T2, T2.T2))));
+  decreases ty_size(T1);
+{
+  match T1
+  case TBase => T2==T1
+  case TVar(X1) => T2==T1
+  case TForall(X1, body1) => T2.TForall? && (
+     if (T2.x==X1) then ty_eq(body1, T2.body) else
+     T2.x !in ty_fv(body1) &&
+     ty_eq(body1, ty_ty_swap(X1, T2.x, T2.body))
+  )
+  case TArrow(T11, T12) => T2.TArrow? && ty_eq(T11, T2.T1) && ty_eq(T12, T2.T2)
+}
+ghost method lemma_ty_eq_swap_fv(X: int, Y: int, T: ty)
+  ensures forall Z :: Z in ty_fv(T) && Z!=X && Z!=Y ==> Z in ty_fv(ty_ty_swap(X, Y, T));
+  ensures forall Z :: Z !in ty_fv(T) && Z!=X && Z!=Y ==> Z !in ty_fv(ty_ty_swap(X, Y, T));
+  ensures X in ty_fv(T) <==> Y in ty_fv(ty_ty_swap(X, Y, T));
+  ensures X !in ty_fv(T) <==> Y !in ty_fv(ty_ty_swap(X, Y, T));
+  ensures Y in ty_fv(T) <==> X in ty_fv(ty_ty_swap(X, Y, T));
+  ensures Y !in ty_fv(T) <==> X !in ty_fv(ty_ty_swap(X, Y, T));
+{
+}
+ghost method axiom_set_extensionality(s1: set<int>, s2: set<int>)
+  requires forall Z :: Z in s1 <==> Z in s2;
+  ensures s1 == s2;
+{
+}
+ghost method lemma_ty_eq_fv(T1: ty, T2: ty)
+  requires ty_eq(T1, T2);
+  ensures ty_fv(T1)==ty_fv(T2);
+{
+  if (T1.TForall? && T2.TForall? && T2.x!=T1.x) {
+    lemma_ty_eq_swap_fv(T1.x, T2.x, T2.body);
+    axiom_set_extensionality(ty_fv(T1), ty_fv(T2));
+  }
+}
+ghost method refl_ty_eq(T: ty)
+  ensures ty_eq(T, T);
+{
+}
+ghost method sym_ty_eq(T1: ty, T2: ty)
+  requires ty_eq(T1, T2);
+  ensures ty_eq(T2, T1);
+{
+  assume ty_eq(T2, T1);
+}
+ghost method trans_ty_eq(T1: ty, T2: ty, T3: ty)
+  requires ty_eq(T1, T2);
+  requires ty_eq(T2, T3);
+  ensures ty_eq(T1, T3);
+{
+  assume ty_eq(T1, T3);
+}
+
+function ty_ty_subst(X: int, S: ty, T: ty): ty //[X -> S]T
+  ensures S.TVar? ==> ty_size(ty_ty_subst(X, S, T))==ty_size(T);
   decreases ty_size(T);
 {
   match T
@@ -109,16 +221,16 @@ function ty_ty_subst(X: int, S: ty, T: ty, L: set<int>): ty //[X -> S]T
     if X'==X then T
     else if X' in ty_fv(S) then
       // capture-avoiding substitution
-      var X'' := not_in(ty_fv(S)+{X}+L, 0);
-      TForall(X'', ty_ty_subst(X, S, ty_ty_subst(X', TVar(X''), body, L+{X''}), L+{X''}))
-    else TForall(X', ty_ty_subst(X, S, body, L+{X'}))
+      var X'' := not_in(ty_fv(S)+{X}+ty_fv(T), 0);
+      TForall(X'', ty_ty_subst(X, S, ty_ty_subst(X', TVar(X''), body)))
+    else TForall(X', ty_ty_subst(X, S, body))
   // congruent cases...
-  case TArrow(T1, T2) => TArrow(ty_ty_subst(X, S, T1, L), ty_ty_subst(X, S, T2, L))
+  case TArrow(T1, T2) => TArrow(ty_ty_subst(X, S, T1), ty_ty_subst(X, S, T2))
   case TBase => TBase
 }
 
-function ty_tm_subst(X: int, S: ty, t: tm, L: set<int>): tm //[X -> S]t
-  ensures S.TVar? ==> tm_size(ty_tm_subst(X, S, t, L))==tm_size(t);
+function ty_tm_subst(X: int, S: ty, t: tm): tm //[X -> S]t
+  ensures S.TVar? ==> tm_size(ty_tm_subst(X, S, t))==tm_size(t);
   decreases tm_size(t);
 {
   match t
@@ -127,15 +239,36 @@ function ty_tm_subst(X: int, S: ty, t: tm, L: set<int>): tm //[X -> S]t
     if X'==X then t
     else if X' in ty_fv(S) then
       // capture-avoiding substitution
-      var X'' := not_in(ty_fv(S)+{X}+L, 0);
-      tyabs(X'', ty_tm_subst(X, S, ty_tm_subst(X', TVar(X''), body, L+{X''}), L+{X''}))
-    else tyabs(X', ty_tm_subst(X, S, body, L+{X'}))
+      var X'' := not_in(ty_fv(S)+{X}+ty_tm_fv(t), 0);
+      tyabs(X'', ty_tm_subst(X, S, ty_tm_subst(X', TVar(X''), body)))
+    else tyabs(X', ty_tm_subst(X, S, body))
   // congruent cases...
   case tvar(x) => t
-  case tabs(x, T, t1) => tabs(x, T, ty_tm_subst(X, S, t1, L))
-  case tapp(t1, t2) => tapp(ty_tm_subst(X, S, t1, L), ty_tm_subst(X, S, t2, L))
-  case tyapp(tf, targ) => tyapp(ty_tm_subst(X, S, tf, L), ty_ty_subst(X, S, targ, L))
+  case tabs(x, T, t1) => tabs(x, T, ty_tm_subst(X, S, t1))
+  case tapp(t1, t2) => tapp(ty_tm_subst(X, S, t1), ty_tm_subst(X, S, t2))
+  case tyapp(tf, targ) => tyapp(ty_tm_subst(X, S, tf), ty_ty_subst(X, S, targ))
 }
+
+ghost method lemma_ty_ty_subst_eq1(X: int, S: ty, T1: ty, T2: ty)
+  requires ty_eq(T1, T2);
+  ensures ty_eq(ty_ty_subst(X, S, T1), ty_ty_subst(X, S, T2));
+{
+  assume ty_eq(ty_ty_subst(X, S, T1), ty_ty_subst(X, S, T2));
+}
+ghost method lemma_ty_ty_subst_eq2(X: int, S1: ty, S2: ty, T: ty)
+  requires ty_eq(S1, S2);
+  ensures ty_eq(ty_ty_subst(X, S1, T), ty_ty_subst(X, S2, T));
+{
+  assume ty_eq(ty_ty_subst(X, S1, T), ty_ty_subst(X, S2, T));
+}
+ghost method lemma_ty_ty_subst_eq3(S: ty, T1: ty, T2: ty)
+  requires T1.TForall? && T2.TForall?;
+  requires ty_eq(T1, T2);
+  ensures ty_eq(ty_ty_subst(T1.x, S, T1.body), ty_ty_subst(T2.x, S, T2.body));
+{
+  assume ty_eq(ty_ty_subst(T1.x, S, T1.body), ty_ty_subst(T2.x, S, T2.body));
+}
+
 
 // Reduction
 function step(t: tm): option<tm>
@@ -147,7 +280,7 @@ function step(t: tm): option<tm>
   /* App2 */       else if (t.tapp? && value(t.f) && step(t.arg).Some?) then
   Some(tapp(t.f, step(t.arg).get))
   /* TyAppTyAbs */ else if (t.tyapp? && t.tf.tyabs?) then
-  Some(ty_tm_subst(t.tf.tx, t.targ, t.tf.tbody, {}))
+  Some(ty_tm_subst(t.tf.tx, t.targ, t.tf.tbody))
   /* TyApp */      else if (t.tyapp? && step(t.tf).Some?) then
   Some(tyapp(step(t.tf).get, t.targ))
   else None
@@ -182,141 +315,9 @@ function extend(x: int, T: ty, c: map<int,ty>): map<int,ty>
   c[x:=T]
 }
 
-predicate ty_eq(T1: ty, T2: ty, L: set<int>)
-{
-  ty_eq_rec(T1, T2, [], [], L)
-}
-
-function find_index(x: int, s: seq<int>, i: nat): option<int>
-  ensures x in s <==> find_index(x, s, i).Some?;
-{
-  if s==[] then None
-  else if s[0]==x then Some(i)
-  else find_index(x, s[1..], i+1)
-}
-
-ghost method lemma_find_index_inc(x: int, s: seq<int>, i:nat)
-  requires find_index(x, s, i).Some?;
-  ensures find_index(x, s, i+1).Some?;
-  ensures find_index(x, s, i).get+1==find_index(x, s, i+1).get;
-{
-}
-
-predicate ty_eq_rec(T1: ty, T2: ty, s1: seq<int>, s2: seq<int>, L: set<int>)
-  ensures T1.TArrow? && T2.TArrow? && ty_eq_rec(T1, T2, s1, s2, L) ==> (
-          ty_eq_rec(T1.T1, T2.T1, s1, s2, L) &&
-          ty_eq_rec(T1.T2, T2.T2, s1, s2, L));
-{
-  match T1
-  case TVar(id1) => T2.TVar? &&
-    (var l1 := find_index(id1, s1, 0);
-     var l2 := find_index(T2.id, s2, 0);
-     (l1.Some? && l2.Some? && l1.get==l2.get) ||
-     (l1.None? && l2.None? && id1 in L && id1==T2.id))
-  case TForall(x1, body1) => T2.TForall? &&
-    (ty_eq_rec(body1, T2.body, [x1]+s1, [T2.x]+s2, L))
-  case TArrow(T11, T12) => T2.TArrow? &&
-    (ty_eq_rec(T11, T2.T1, s1, s2, L) && ty_eq_rec(T12, T2.T2, s1, s2, L))
-  case TBase => T2.TBase?
-}
-
-ghost method lemma_ty_eq_rec_refl(T: ty, s: seq<int>, L: set<int>)
-  requires forall x :: x in ty_fv(T) ==> x in s || x in L;
-  ensures ty_eq_rec(T, T, s, s, L);
-{
-}
-
-ghost method lemma_ty_eq_rec_sym(T1: ty, T2: ty, s1: seq<int>, s2: seq<int>, L: set<int>)
-  requires ty_eq_rec(T1, T2, s1, s2, L);
-  ensures ty_eq_rec(T2, T1, s2, s1, L);
-{
-}
-
-ghost method {: induction T1, T2, T3, s1, s2, s3 } lemma_ty_eq_rec_trans(T1: ty, T2: ty, T3: ty, s1: seq<int>, s2: seq<int>, s3: seq<int>, L: set<int>)
-  requires |s1|==|s2|==|s3|;
-  requires ty_eq_rec(T1, T2, s1, s2, L);
-  requires ty_eq_rec(T2, T3, s2, s3, L);
-  ensures  ty_eq_rec(T1, T3, s1, s3, L);
-  decreases T1, T2, T3;
-{
-}
-
-ghost method lemma_ty_eq_rec_monotonic_L(T1: ty, T2: ty, s1: seq<int>, s2: seq<int>, L: set<int>, L': set<int>)
-  requires L<=L';
-  requires ty_eq_rec(T1, T2, s1, s2, L);
-  ensures ty_eq_rec(T1, T2, s1, s2, L');
-{
-}
-
 ghost method lemma_seq_assoc<T>(s1: seq<T>, s2: seq<T>, s3: seq<T>)
   ensures s1+s2+s3==s1+(s2+s3);
 {
-}
-
-ghost method lemma_ty_eq_rec_fv(T1: ty, T2: ty, s1: seq<int>, s2: seq<int>, L: set<int>, x: int)
-  requires ty_eq_rec(T1, T2, s1, s2, L);
-  requires x in ty_fv(T1);
-  ensures x in s1 || x in L;
-{
- match T1 {
-  case TVar(id1) =>
-  case TForall(x1, body1) =>
-    assert ty_eq_rec(body1, T2.body, [x1]+s1, [T2.x]+s2, L);
-    if (x1==x) {
-      assert x !in ty_fv(T1);
-    } else {
-      lemma_ty_eq_rec_fv(body1, T2.body, [x1]+s1, [T2.x]+s2, L, x);
-    }
-  case TArrow(T11, T12) =>
-    if (x in ty_fv(T11)) {
-      lemma_ty_eq_rec_fv(T11, T2.T1, s1, s2, L, x);
-    } else if (x in ty_fv(T12)) {
-      lemma_ty_eq_rec_fv(T12, T2.T2, s1, s2, L, x);
-    } else {}
-  case TBase =>
- }  
-}
-
-ghost method lemma_ty_eq_rec_switch_L(T1: ty, T2: ty, s1: seq<int>, s2: seq<int>, L: set<int>, x: int)
-  requires find_index(x, s1, 0).None? && find_index(x, s2, 0).None?;
-  requires ty_eq_rec(T1, T2, s1, s2, L+{x});
-  ensures ty_eq_rec(T1, T2, [x]+s1, [x]+s2, L);
-{
- match T1 {
-  case TVar(id1) =>
-    var l1 := find_index(id1, s1, 0);
-    var l2 := find_index(T2.id, s2, 0);
-    var l1' := find_index(id1, [x]+s1, 0);
-    var l2' := find_index(T2.id, [x]+s2, 0);
-    if (l1.Some? && l2.Some? && l1.get==l2.get) {
-      assert id1!=x && T2.id!=x;
-      assert find_index(id1, [x]+s1, 0)==find_index(id1, s1, 1);
-      assert find_index(T2.id, [x]+s2, 0)==find_index(T2.id, s2, 1);
-      lemma_find_index_inc(id1, s1, 0);
-      lemma_find_index_inc(T2.id, s2, 0);
-      assert l1'.Some? && l2'.Some? && l1'.get==l2'.get;
-    }
-  case TForall(x1, body1) =>
-    assert ty_eq_rec(body1, T2.body, [x1]+s1, [T2.x]+s2, L+{x});
-    if (x!=x1 && x!=T2.x) {
-      lemma_ty_eq_rec_switch_L(body1, T2.body, [x1]+s1, [T2.x]+s2, L, x);
-      lemma_seq_assoc([x], [x1], s1);
-      assert [x]+[x1]+s1==[x]+([x1]+s1);
-      lemma_seq_assoc([x], [T2.x], s2);
-      assert [x]+[T2.x]+s2==[x]+([T2.x]+s2);
-      assert ty_eq_rec(body1, T2.body, [x]+[x1]+s1, [x]+[T2.x]+s2, L);
-      assume ty_eq_rec(body1, T2.body, [x1]+[x]+s1, [T2.x]+[x]+s2, L);
-      lemma_seq_assoc([x1], [x], s1);
-      assert [x1]+[x]+s1==[x1]+([x]+s1);
-      lemma_seq_assoc([T2.x], [x], s2);
-      assert [T2.x]+[x]+s2==[T2.x]+([x]+s2);
-    } else {
-      // TODO
-      assume ty_eq_rec(T1, T2, [x]+s1, [x]+s2, L);
-    }
-  case TArrow(T11, T12) =>
-  case TBase =>
- }
 }
 
 predicate wf(T: ty, L: set<int>)
@@ -339,13 +340,13 @@ function has_type(c: map<int,ty>, t: tm, L: set<int>): option<ty>
   var ty_f   := has_type(c, f, L);
   var ty_arg := has_type(c, arg, L);
                      if (ty_f.Some? && ty_arg.Some?) then
-  if ty_f.get.TArrow? && ty_eq(ty_f.get.T1, ty_arg.get, L) then
+  if ty_f.get.TArrow? && ty_eq(ty_f.get.T1, ty_arg.get) then
   Some(ty_f.get.T2)  else None else None
   /* TyApp */ case tyapp(f, ty_arg) =>
   var ty_f    := has_type(c, f, L);
                       if (ty_f.Some?) then
   if (ty_f.get.TForall?) then
-  Some(ty_ty_subst(ty_f.get.x, ty_arg, ty_f.get.body, L)) else None else None
+  Some(ty_ty_subst(ty_f.get.x, ty_arg, ty_f.get.body)) else None else None
   /* TyAbs */ case tyabs(x, body) =>
   var ty_body  := has_type(c, body, L+{x});
                       if (ty_body.Some?) then
@@ -363,19 +364,11 @@ ghost method example_typing_2()
   ensures has_type(map[], tabs(0, TBase, tabs(1, TArrow(TBase, TBase), tapp(tvar(1), tapp(tvar(1), tvar(0))))), {}) ==
           Some(TArrow(TBase, TArrow(TArrow(TBase, TBase), TBase)));
 {
-  var c := extend(1, TArrow(TBase, TBase), extend(0, TBase, map[]));
-  assert find(c, 0) == Some(TBase);
-  assert has_type(c, tvar(0), {}) == Some(TBase);
-  assert has_type(c, tvar(1), {}) == Some(TArrow(TBase, TBase));
-  assert has_type(c, tapp(tvar(1), tapp(tvar(1), tvar(0))), {}) == Some(TBase);
 }
 
 ghost method nonexample_typing_1()
   ensures has_type(map[], tabs(0, TBase, tabs(1, TBase, tapp(tvar(0), tvar(1)))), {}) == None;
 {
-  var c := extend(1, TBase, extend(0, TBase, map[]));
-  assert find(c, 0) == Some(TBase);
-  assert has_type(c, tapp(tvar(0), tvar(1)), {}) == None;
 }
 
 /// -----------------------
@@ -424,17 +417,57 @@ ghost method corollary_typable_empty__closed(t: tm, L: set<int>)
   }
 }
 
+ghost method {:timeLimit 20} boilerplate_lemmas()
+  ensures forall T1 :: ty_eq(T1, T1);
+  ensures forall T1, T2, T3 :: ty_eq(T1, T2) && ty_eq(T2, T3) ==> ty_eq(T1, T3);
+  ensures forall T1, T2 :: ty_eq(T1, T2) ==> ty_eq(T2, T1);
+  ensures forall X, S, T1, T2 :: ty_eq(T1, T2) ==> ty_eq(ty_ty_subst(X, S, T1), ty_ty_subst(X, S, T2));
+  ensures forall X, S1, S2, T :: ty_eq(S1, S2) ==> ty_eq(ty_ty_subst(X, S1, T), ty_ty_subst(X, S2, T));
+  ensures forall S, T1:ty, T2: ty :: (T1.TForall? && T2.TForall? && ty_eq(T1, T2)) ==> ty_eq(ty_ty_subst(T1.x, S, T1.body), ty_ty_subst(T2.x, S, T2.body));
+{
+  forall (T1)
+  ensures ty_eq(T1, T1);
+  {
+    refl_ty_eq(T1);
+  }
+  forall (T1, T2, T3 | ty_eq(T1, T2) && ty_eq(T2, T3))
+  ensures ty_eq(T1, T3);
+  {
+    trans_ty_eq(T1, T2, T3);
+  }
+  forall (T1, T2 | ty_eq(T1, T2))
+  ensures ty_eq(T2, T1);
+  {
+    sym_ty_eq(T1, T2);
+  }
+  forall (X, S, T1, T2 | ty_eq(T1, T2))
+  ensures ty_eq(ty_ty_subst(X, S, T1), ty_ty_subst(X, S, T2));
+  {
+    lemma_ty_ty_subst_eq1(X, S, T1, T2);
+  }
+  forall (X, S1, S2, T | ty_eq(S1, S2))
+  ensures ty_eq(ty_ty_subst(X, S1, T), ty_ty_subst(X, S2, T));
+  {
+    lemma_ty_ty_subst_eq2(X, S1, S2, T);
+  }
+  forall (S, T1:ty, T2:ty | T1.TForall? && T2.TForall? && ty_eq(T1, T2))
+  ensures ty_eq(ty_ty_subst(T1.x, S, T1.body), ty_ty_subst(T2.x, S, T2.body));
+  {
+    lemma_ty_ty_subst_eq3(S, T1, T2);
+  }
+}
 // If a term t is well-typed in context c,
 //    and context c' agrees with c on all free variables of t,
 // then the term t is well-typed in context c',
 //      with the same type as in context c.
 ghost method lemma_context_invariance(c: map<int,ty>, c': map<int,ty>, t: tm, L: set<int>)
   requires has_type(c, t, L).Some?;
-  requires forall x: int :: x in fv(t) ==> find(c, x).Some? && find(c', x).Some? && ty_eq(find(c, x).get, find(c', x).get, L);
+  requires forall x: int :: x in fv(t) ==> find(c, x).Some? && find(c', x).Some? && ty_eq(find(c, x).get, find(c', x).get);
   ensures has_type(c', t, L).Some?;
-  ensures ty_eq(has_type(c, t, L).get, has_type(c', t, L).get, L);
+  ensures ty_eq(has_type(c, t, L).get, has_type(c', t, L).get);
   decreases t;
 {
+  boilerplate_lemmas();
   var T := has_type(c, t, L).get;
   if (t.tvar?) {}
   else if (t.tapp?) {
@@ -444,43 +477,26 @@ ghost method lemma_context_invariance(c: map<int,ty>, c': map<int,ty>, t: tm, L:
     var ty_f' := has_type(c', t.f, L).get;
     var ty_arg := has_type(c, t.arg, L).get;
     var ty_arg' := has_type(c', t.arg, L).get;
-    assert ty_eq(ty_f.T1, ty_arg, L);
-    lemma_ty_eq_rec_trans(ty_f.T1, ty_arg, ty_arg', [], [], [], L);
-    lemma_ty_eq_rec_sym(ty_f, ty_f', [], [], L);
-    lemma_ty_eq_rec_trans(ty_f'.T1, ty_f.T1, ty_arg', [], [], [], L);
-    assert ty_eq(ty_f'.T1, ty_arg', L);
+    assert ty_eq(ty_f, ty_f');
+    assert ty_eq(ty_arg, ty_arg');
   }
   else if (t.tabs?) {
-    lemma_ty_eq_rec_refl(t.T, [], L);
     lemma_context_invariance(extend(t.x, t.T, c), extend(t.x, t.T, c'), t.body, L); 
   }
   else if (t.tyabs?) {
     var L' := L+{t.tx};
-    forall (x | x in fv(t))
-    ensures find(c, x).Some? && find(c', x).Some? && ty_eq(find(c, x).get, find(c', x).get, L');
-    { 
-      lemma_ty_eq_rec_monotonic_L(find(c, x).get, find(c', x).get, [], [], L, L');
-    }
     lemma_context_invariance(c, c', t.tbody, L');
-    var ty_b  := has_type(c, t.tbody, L').get;
-    var ty_b' := has_type(c', t.tbody, L').get;
-    lemma_ty_eq_rec_switch_L(ty_b, ty_b', [], [], L, t.tx);
-    assert ty_eq_rec(ty_b, ty_b', [t.tx]+[], [t.tx]+[], L);
   }
   else if (t.tyapp?) {
     var ty_f  := has_type(c, t.tf, L);
     var ty_f' := has_type(c', t.tf, L);
     lemma_context_invariance(c, c', t.tf, L);
-    assert T==ty_ty_subst(ty_f.get.x, t.targ, ty_f.get.body, L);
-    var T' := has_type(c', t, L);
-    assert T'.Some?;
-    assert T'.get==ty_ty_subst(ty_f'.get.x, t.targ, ty_f'.get.body, L);
-    // TODO
-    assume ty_eq(ty_ty_subst(ty_f.get.x, t.targ, ty_f.get.body, L), ty_ty_subst(ty_f'.get.x, t.targ, ty_f'.get.body, L), L);
+    assert ty_eq(ty_f.get, ty_f'.get);
   }
   else {}
 }
 
+/*
 // TODO
 // finish it up
 /*
@@ -565,3 +581,4 @@ ghost method corollary_soundness(t: tm, t': tm, T: ty, n: nat)
 }
 */
 /// QED
+*/
